Refactor common code of greedy constructions (#939)
The greedy methods for 1076, 1722, 3308 share a lot of similarities, so
we could try to reduce the code doubling.

Closes #771

equational_theories/ManuallyProved/Equation1076.lean
@@ -7,200 +7,34 @@ import Mathlib.Data.Set.Finite.Lattice
 import Mathlib.Data.Set.Basic
 import Mathlib.Data.Set.Functor
 import Mathlib.Tactic.DeriveFintype
-
+import equational_theories.AdjoinFresh
 import equational_theories.Equations.All
 import equational_theories.FactsSyntax
+import equational_theories.PartialMagma
 
 import Mathlib.Data.FinEnum
 
 namespace Eq1076
 namespace Greedy
 noncomputable section
+open AdjoinFresh PartialMagma
 
---TODO: find better name
-def adjoinFresh' {F : Type} [fE: FinEnum F]: ℕ ≃ ℕ ⊕ F where
-  toFun n := if h: n < fE.card then .inr $ fE.equiv.symm ⟨n,h⟩ else .inl $ n - fE.card
-  invFun a := match a with
-  | .inl n => n + fE.card
-  | .inr f => fE.equiv f
-  left_inv n := by
-    simp only
-    split
-    case h_1 h =>
-      split at h
-      · injection h
-      · injection h
-        omega
-    case h_2 h =>
-      split at h
-      · injection h with h
-        rw [← h]
-        simp
-      · injection h
-  right_inv a := by cases a <;> simp
 
-def adjoinFresh {F : Type} (e : ℕ ≃ ℕ ⊕ F) (m : ℕ) : ℕ ≃ ℕ ⊕ F where
-  toFun n := if n < m then .inl n else match e (n - m) with
-    | .inl k => .inl (k + m)
-    | .inr c => .inr c
-  invFun
-    | .inl k => if k < m then k else e.symm (.inl (k-m)) + m
-    | .inr c => e.symm (.inr c) + m
-  left_inv n := by
-    dsimp
-    by_cases h : n < m
-    · simp [h]
-    · simp [h]
-      split
-      cases h' : e (n -m)
-      next k' eq' k'' =>
-        rw [h'] at eq'
-        simp only [Sum.inl.injEq] at eq'
-        rw [← eq']
-        have  : ¬ k'' + m < m := by omega
-        simp only [this, ↓reduceIte, Nat.add_sub_cancel]
-        rw [← h']
-        simp only [Equiv.symm_apply_apply]
-        omega
-      · simp_all
-      next h' =>
-        split at h'
-        · simp_all
-        next h'' =>
-          rw [← h',← h'']
-          simp only [Equiv.symm_apply_apply]
-          omega
-  right_inv a := by
-    cases a
-    case inl n =>
-      simp only
-      by_cases h : n < m
-      · simp [h]
-      · simp only [h, ↓reduceIte, Nat.add_sub_cancel, Equiv.apply_symm_apply]
-        have : ¬ (e.symm (Sum.inl (n - m)) + m < m) := by omega
-        simp only [this, ↓reduceIte, Sum.inl.injEq]
-        omega
-    case inr => simp
-
-theorem adjoinFresh_fixed {F : Type} {e : ℕ ≃ ℕ ⊕ F} {m k: ℕ} (h : k  < m) :
-  adjoinFresh e m k = .inl k := by unfold adjoinFresh ; simp [h]
-
-theorem adjoinFresh_fixed' {F : Type} {e : ℕ ≃ ℕ ⊕ F} {m k: ℕ} (h : k  < m) :
-  (adjoinFresh e m).symm (.inl k) = k := by unfold adjoinFresh ; simp [h]
-
-abbrev PreExtension (α : Type) := α → α → Set α
-
-structure PreExtension.OK {α : Type} (E : PreExtension α) : Prop where
-  finite : Set.Finite {x : (α × α) × α | x.2 ∈ E x.1.1 x.1.2}
-  func {x y} : Set.Subsingleton (E x y)
+structure Laws {α : Type} (E : PreExtension α) : Prop where
   eq1076 {x y xy xxy} : xy ∈ E x y → xxy ∈ E x xy → ∃xxyy, xxyy ∈ E xxy y ∧ x ∈ E y xxyy
   not_idempotent {x} : x ∉ E x x
 
-private abbrev Equiv.movePreExtension {α β : Type} (e : α ≃ β) (E : PreExtension β) : PreExtension α :=
-  fun a b => { c | e c ∈ E (e a) (e b) }
 
-def Equiv.movePreExtensionOK {α β : Type} (e : α ≃ β) (E : PreExtension β) (ok : E.OK) :
-  (Equiv.movePreExtension e E).OK where
-  finite := by
-    apply ok.finite.of_equiv
-    constructor
-    case toFun =>
-      refine fun ⟨((a,b),c),h⟩ => ⟨((e.symm a, e.symm b),e.symm c),?_⟩
-      simp_all
-    case invFun =>
-      refine fun ⟨((a,b),c),h⟩ => ⟨((e a, e b),e c),?_⟩
-      simp_all
-    case left_inv =>
-      refine fun ⟨((a,b),c),h⟩ => ?_
-      simp_all
-    case right_inv =>
-      refine fun ⟨((a,b),c),h⟩ => ?_
-      simp_all
-  func {x y} z z_mem z' z'_mem := by
-    have := ok.func z_mem z'_mem
-    simpa
+def Laws_equiv {α β : Type} (e : α ≃ β) (E : PreExtension β) (ok : Laws E) :
+  Laws (Equiv.movePreExtension e E) where
   eq1076 xy_mem xxy_mem := by
     obtain ⟨xxyy, xxyy_mem, eq⟩ := ok.eq1076 xy_mem xxy_mem
     exact ⟨e.symm xxyy, by simpa using xxyy_mem, by simpa using eq⟩
   not_idempotent h := by simpa using ok.not_idempotent (by simpa using h)
 
-
-
-abbrev Extension α:= {E : PreExtension α // E.OK}
-
-class ExtensionBase where
-  E : PreExtension ℕ
-  ok : E.OK
-  a : ℕ
-  b : ℕ
-  not_def {c} : c ∉ E a b
-
-namespace ExtensionBase
-variable [ExtensionBase]
-
--- Not show how to call this
-structure FreshSolution (F : Type) (E' : PreExtension (ℕ ⊕ F)) : Prop where
-  base {a b c} : c ∈ E a b → (.inl c) ∈ E' (.inl a) (.inl b)
-  ok : E'.OK
-  ab_def : (E' (.inl a) (.inl b)).Nonempty
-
-abbrev FreshExtension (F : Type) := {E' : PreExtension (ℕ ⊕ F) // FreshSolution F E'}
-
-scoped infix:80 " ◯ " => E
-def dom : Finset ℕ :=
-  insert a <| insert b <| ok.finite.toFinset.biUnion fun ((a, b), c) => {a, b, c}
-
-theorem mem_dom {a b c x}
-    (h1 : c ∈ a ◯ b) (h2 : x ∈ ({a, b, c} : Finset ℕ)) : x ∈ dom := by
-  refine Finset.mem_insert_of_mem <| Finset.mem_insert_of_mem ?_
-  simp only [dom, Finset.mem_biUnion, Set.Finite.mem_toFinset, Set.mem_setOf_eq, Prod.exists]
-  exact ⟨_, _, _, h1, h2⟩
-
-@[scoped aesop safe forward]
-theorem dom_l {a b c} (h : c ∈ a ◯ b) : a ∈ dom := mem_dom h (by simp)
-@[scoped aesop safe forward]
-theorem dom_r {a b c} (h : c ∈ a ◯ b) : b ∈ dom := mem_dom h (by simp)
-@[scoped aesop safe forward]
-theorem dom_o {a b c} (h : c ∈ a ◯ b) : c ∈ dom := mem_dom h (by simp)
-@[scoped aesop safe forward]
-theorem dom_a : a ∈ dom := Finset.mem_insert_self ..
-@[scoped aesop safe forward]
-theorem dom_b : b ∈ dom := Finset.mem_insert_of_mem <| Finset.mem_insert_self ..
-
-def dom_bound := dom.sup id + 1
-
-theorem lt_dom_bound {x} (h : x ∈ dom) : x < dom_bound := Nat.lt_succ.2 <| dom.le_sup (f := id) h
-
-namespace FreshExtension
-
-variable {F : Type} [FinEnum F] (E' : FreshExtension F)
-
-def adjoin : PreExtension ℕ :=
-  Equiv.movePreExtension (adjoinFresh adjoinFresh' dom_bound) E'.1
-
-theorem adjoin_ok : E'.adjoin.OK :=
-  Equiv.movePreExtensionOK (adjoinFresh adjoinFresh' dom_bound) E'.1 E'.2.ok
-
-theorem adjoin_le : E ≤ E'.adjoin := by
-  intro a b c h
-  unfold adjoin Equiv.movePreExtension
-  simp only [Set.mem_setOf_eq]
-  unfold adjoinFresh
-  simp only [Equiv.coe_fn_mk, lt_dom_bound (dom_l h), ↓reduceIte, lt_dom_bound (dom_r h),
-    lt_dom_bound (dom_o h)]
-  exact E'.2.base h
-
-theorem adjoin_ab_def :
-  E'.adjoin ∈ { e : (PreExtension ℕ) | Nonempty (e a b)} := by
-  obtain ⟨c, c_mem⟩ := E'.2.ab_def
-  use ((adjoinFresh adjoinFresh' dom_bound).symm c)
-  unfold adjoin Equiv.movePreExtension
-  simp only [Set.mem_setOf_eq, Equiv.apply_symm_apply]
-  unfold adjoinFresh
-  simp [lt_dom_bound dom_a, lt_dom_bound dom_b, c_mem]
-
-end FreshExtension
-end ExtensionBase
+scoped instance : ExtensionRules where
+  laws := Laws
+  laws_equiv := Laws_equiv
 
 --no extra assumptions, keep this to be consistent with other methods
 class Extension1 extends ExtensionBase where
@@ -214,8 +48,6 @@ open ExtensionBase
 The unit corresponds to c, the first Fin to c'ᵢ, the second one to c''ᵢ.
 To easily infer FinEnum we keep it as is, might also be possible to define an inductive type instead -/
 private abbrev F := Unit ⊕ Fin dom_bound ⊕ Fin dom_bound
-
-example : FinEnum F := by infer_instance
 
 open ExtensionBase
 --unfold constructors to get better pattern matching
@@ -257,9 +89,9 @@ theorem next_not_idempotent {x y} : x = y → x ∉ next x y := by
   case base h =>
     simp only [Sum.inl.injEq] at eq
     rw [eq] at h
-    apply ok.not_idempotent h
+    apply ok.laws.not_idempotent h
   case extra4_2 h =>
-    apply ok.not_idempotent h
+    apply ok.laws.not_idempotent h
   case extra2 => injection eq
 
 theorem next_eq1076 {x y xy xxy} : xy ∈ next x y → xxy ∈ next x xy → ∃xxyy, xxyy ∈ next xxy y ∧ x ∈ next y xxyy := by
@@ -269,7 +101,7 @@ theorem next_eq1076 {x y xy xxy} : xy ∈ next x y → xxy ∈ next x xy → ∃
     <;> generalize hb : b = b' at *
     <;> cases xxy_mem
   case base.base xy_mem _ xxy_mem =>
-    obtain ⟨xxyy, xxyy_mem, eq⟩ := ok.eq1076 xy_mem xxy_mem
+    obtain ⟨xxyy, xxyy_mem, eq⟩ := ok.laws.eq1076 xy_mem xxy_mem
     exact ⟨.inl xxyy, .base xxyy_mem, .base eq⟩
   case base.new h =>
     exact ⟨_, .extra1 h, .extra2 h⟩
@@ -280,9 +112,9 @@ theorem next_eq1076 {x y xy xxy} : xy ∈ next x y → xxy ∈ next x xy → ∃
     · exact ⟨_, .extra3_2 h eq h', .extra3_1 h eq h'⟩
   case extra2.new h =>
     rw [ha, hb] at h
-    exact (ok.not_idempotent h).elim
-  case extra3_1.extra4_1 h => exact (ok.not_idempotent h).elim
-  case extra4_1.extra4_1 h => exact (ok.not_idempotent h).elim
+    exact (ok.laws.not_idempotent h).elim
+  case extra3_1.extra4_1 h => exact (ok.laws.not_idempotent h).elim
+  case extra4_1.extra4_1 h => exact (ok.laws.not_idempotent h).elim
   case extra4_2.new h _ => exact (not_def h).elim
   case extra4_2.base d d_mem h e h' =>
     have eq : d = e := ok.func d_mem h'
@@ -303,9 +135,10 @@ theorem next_ok : next.OK where
     | extra3_2 h _ h' => simp [dom_a, dom_b, dom_r h, dom_o h']
     | _ h => simp [dom_a, dom_b, dom_r h]
   func {x y xy} hxy {xy'} hxy' := next_func hxy hxy'
+  laws := {
   not_idempotent := next_not_idempotent rfl
   eq1076 := next_eq1076
-
+  }
 def next_freshSolution : FreshSolution F Next where
   base := Next.base
   ok := next_ok
@@ -343,7 +176,7 @@ theorem exists_extension :
     replace le a ha := Finset.forall_image.1 le a ha _ _ (hop a.1 a.2)
     simp only [Finset.mem_insert, Finset.mem_singleton, forall_eq_or_imp, forall_eq, S] at le
     obtain ⟨xy, xxy, xxyy, final⟩ := le
-    obtain ⟨xxyy', xxyy'_def, eq⟩ := (e.2.eq1076 xy xxy)
+    obtain ⟨xxyy', xxyy'_def, eq⟩ := (e.2.laws.eq1076 xy xxy)
     exact e.2.func eq ((e.2.func xxyy xxyy'_def) ▸ final)
   · exact (hf1 ..).func (h2 _ (hf2 x y) _ _ H) (hop ..)
 
@@ -354,9 +187,8 @@ instance (n) : OfNat (GreedyMagma e₀) n := inferInstanceAs (OfNat Nat n)
 noncomputable instance instMagma : Magma (GreedyMagma e₀) where
   op := (exists_extension e₀).choose
 
-theorem Extension.eq1076 : Equation1076 (GreedyMagma e₀) :=
+theorem _root_.PartialMagma.Extension.eq1076 : Equation1076 (GreedyMagma e₀) :=
   (exists_extension e₀).choose_spec.1
-
 
 theorem Extension.base : ∀ {x y z : GreedyMagma e₀}, z ∈ e₀.1 x y → z = x ◇ y :=
   (exists_extension e₀).choose_spec.2
@@ -374,7 +206,8 @@ theorem fromList_ok {S : List ((Nat ×ₗ Nat) × Nat)}
     have : IsTrans ((ℕ ×ₗ ℕ) × ℕ) (·.1 < ·.1) := ⟨fun _ _ _ => lt_trans⟩
     (List.chain'_iff_pairwise.1 sorted) |>.imp (fun h => h.ne)
       |>.forall (fun _ _ => (·.symm)) h1 h2 (by rintro ⟨⟩; exact h rfl) rfl
-  eq1076 h1 h2 := by -- variable names are off, copy pase from 1722 just worked
+  laws := {
+  eq1076 := fun h1 h2 => by -- variable names are off, copy pase from 1722 just worked
     obtain ⟨⟨⟨y, y'⟩,yy⟩, yy_mem, ⟨⟨yy', xyy⟩,x⟩, eq_mem, y_def,
     y'_def, yy'_def, xyy_def, x_def⟩ := eq1076 _ h1 _ h2 rfl rfl
     simp only at yy_mem eq_mem y_def y'_def yy_mem yy'_def xyy_def x_def
@@ -382,8 +215,8 @@ theorem fromList_ok {S : List ((Nat ×ₗ Nat) × Nat)}
     rewrite [y_def, y'_def] at yy_mem
     use yy_mem
     use yy'_def ▸xyy_def ▸ x_def ▸ eq_mem
-  not_idempotent h := not_idempotent _ h rfl rfl
-
+  not_idempotent := fun h => not_idempotent _ h rfl rfl
+  }
 
 theorem fromList_eval {e : Extension ℕ} {S : List ((Nat × Nat) × Nat)} (hS : e.1 = fromList S)
     (a b c : Nat) (h : ((a, b), c) ∈ S := by decide) :
@@ -397,7 +230,7 @@ theorem fromList_eval' {e : Extension ℕ} {S : List ((Nat × Nat) × Nat)} (hS 
 
 end
 end Greedy
-open Greedy
+open Greedy PartialMagma
 /-- see https://leanprover.zulipchat.com/#narrow/channel/458659-Equational/topic/713.2C.201289.2C.201447/near/483735768
 for the seed data -/
 
