equational_theories/ManuallyProved.lean
@@ -1,4 +1,5 @@
 import equational_theories.ManuallyProved.Equation73
+import equational_theories.ManuallyProved.Equation713
 import equational_theories.ManuallyProved.Equation854
 import equational_theories.ManuallyProved.Equation917
 import equational_theories.ManuallyProved.Equation1076
